Extensional tensor (#47)
* [WIP] checkpoint tensor2d developments

* fix scoping rules

* Cleanup KDTensor.

* nat lemma: 0 < x => x cancellable

* fixup: revive rewrite theorem

* add TODO about state

MLIR/Semantics/Semantics.lean
@@ -56,17 +56,27 @@ inductive IOp (δ: Dialect α σ ε) := | mk
   (name:    String) -- TODO: name should come from an Enum in δ.
   (resTy:   List (MLIRType δ))
   (args:    TypedArgs δ)
-  (regions: List (TypedArgs δ → OpM δ (TypedArgs δ))) -- TODO: surely, I can build the denotation of a region and pass it along to you?
+  (regions: List (TypedArgs δ → OpM δ (TypedArgs δ)))
   (attrs:   AttrDict δ)
 
 
 -- The monad in which these computations are run
-abbrev TopM (Δ: Dialect α σ ε) (R: Type _) := StateT (SSAEnv Δ) (Except String) R
-def TopM.run (t: TopM Δ R) (env: SSAEnv Δ): Except String (R × SSAEnv Δ) :=
+abbrev TopM (Δ: Dialect α σ ε) (R: Type _) := StateT (SSAEnv Δ) (Except (String × (SSAEnv Δ))) R
+def TopM.run (t: TopM Δ R) (env: SSAEnv Δ): Except (String × (SSAEnv Δ)) (R × SSAEnv Δ) :=
   StateT.run t env
 
-def TopM.raiseUB {Δ: Dialect α σ ε} (message: String): TopM Δ R :=
-  Except.error message
+def TopM.scoped (t: TopM Δ R): TopM Δ R := do
+  -- TODO: convert this to using the `SSAEnv`'s ability to a stack of `SSAScope`,
+  -- instead of approximating it with overwriting the `SSAEnv` temporarily.
+  let state ← get -- save scope
+  let res ← t -- run computation
+  set state -- restore scope
+  return res -- return result
+
+
+def TopM.raiseUB {Δ: Dialect α σ ε} (message: String): TopM Δ R := do
+  let state ← get
+  Except.error (message, state)
 
 def TopM.get {Δ: Dialect α σ ε} (τ: MLIRType Δ) (name: SSAVal): TopM Δ τ.eval := do
   let s ← StateT.get
@@ -76,9 +86,22 @@ def TopM.get {Δ: Dialect α σ ε} (τ: MLIRType Δ) (name: SSAVal): TopM Δ τ
 
 def TopM.set {Δ: Dialect α σ ε} (τ: MLIRType Δ) (name: SSAVal) (v: τ.eval): TopM Δ Unit := do
   let s ← StateT.get
-  StateT.set (SSAEnv.set name τ v s)
+  match SSAEnv.get name τ s with
+  | .some v' => if v == v' then pure () else TopM.raiseUB "setting to SSA value twice!"
+  | .none => StateT.set (SSAEnv.set name τ v s)
 
 
+/-
+TODO:
+
+theorem raiseUB_commutes
+theorem set_commutes_noninterfereing_set
+theorem set_commutes_noninterfereing_get
+theorem set_interference_ub
+theorem set_commutes_set:
+theorem get_commutes_get
+theorem get_commutes_noninterfering_set
+-/
 
 class Semantics (Δ: Dialect α σ ε)  where
   -- Operation semantics function: maps an IOp (morally an Op but slightly less
@@ -111,22 +134,22 @@ def denoteTypedArgs (args: TypedArgs Δ) (names: List SSAVal): TopM Δ Unit :=
         denoteTypedArgs args names
 
 -- Denote a region with an abstract `OpM.RunRegion`
-def denoteRegionOpM {Δ: Dialect α σ ε}
+def OpM.denoteRegion {Δ: Dialect α σ ε}
   (_r: Region Δ)
   (ix: Nat): TypedArgs Δ → OpM Δ (TypedArgs Δ) :=
    fun args => OpM.RunRegion ix args (fun retvals => OpM.Ret retvals)
 
 -- Denote the list of regions with an abstract `OpM.runRegion`
-def denoteRegionsOpM {Δ: Dialect α σ ε}
+def OpM.denoteRegions {Δ: Dialect α σ ε}
   (regions: List (Region Δ))
   (ix: Nat): List (TypedArgs Δ → OpM Δ (TypedArgs Δ)) :=
  match regions with
  | [] => []
- | r :: rs => (denoteRegionOpM r ix) :: denoteRegionsOpM rs (ix + 1)
+ | r :: rs => (OpM.denoteRegion r ix) :: OpM.denoteRegions rs (ix + 1)
 
 -- Denote a region by using its denotation function from the list
 -- of regions. TODO: refactor to use Option
-def denoteRegionByIx
+def TopM.denoteRegionsByIx
   (rs0: List (TypedArgs Δ → TopM Δ (TypedArgs Δ)))
  (ix: Nat) (args: TypedArgs Δ): TopM Δ (TypedArgs Δ) :=
   match rs0 with
@@ -134,7 +157,7 @@ def denoteRegionByIx
   | r:: rs' =>
     match ix with
     | 0 => r args
-    | ix' + 1 => denoteRegionByIx rs' ix' args
+    | ix' + 1 => TopM.denoteRegionsByIx rs' ix' args
 
 -- Morphism from OpM to topM
 def OpM.toTopM (rs0: List (TypedArgs Δ → TopM Δ (TypedArgs Δ))):
@@ -143,60 +166,47 @@ def OpM.toTopM (rs0: List (TypedArgs Δ → TopM Δ (TypedArgs Δ))):
 | OpM.Ret r => pure r
 | OpM.Error s => TopM.raiseUB s
 | OpM.RunRegion ix args k => do
-       let ret <- denoteRegionByIx rs0 ix args
+       let ret <- TopM.denoteRegionsByIx rs0 ix args
        OpM.toTopM rs0 (k ret)
-
 mutual
 variable (Δ: Dialect α' σ' ε') [S: Semantics Δ]
 
 -- unfolded version of List.map denoteRegion.
 -- This allows the termination checker to view the termination.
-def mapDenoteRegion:
+def TopM.mapDenoteRegion:
   List (Region Δ) →
   List (TypedArgs Δ → TopM Δ (TypedArgs Δ))
 | [] => []
-| r :: rs => (denoteRegion r) :: mapDenoteRegion rs
+| r :: rs => (TopM.scoped ∘ denoteRegion r) :: TopM.mapDenoteRegion rs
 
 -- Convert a region to its denotation to establish finiteness.
 -- Then use this finiteness condition to evaluate region semantics.
 -- Use the morphism from OpM to TopM.
-def denoteOp (op: Op Δ) (terminator: Bool):
+def denoteOp (op: Op Δ):
     TopM Δ (TypedArgs Δ) :=
   match op with
   | .mk name res0 args0 regions0 attrs => do
-      let regionSemantics := mapDenoteRegion regions0
       let resTy := res0.map Prod.snd
       let args ← args0.mapM (fun (name, τ) => do
         pure ⟨τ, ← TopM.get τ name⟩)
       -- Built the interpreted operation
-      let iop : IOp Δ := IOp.mk name resTy args (denoteRegionsOpM regions0 0) attrs
+      let iop : IOp Δ := IOp.mk name resTy args (OpM.denoteRegions regions0 0) attrs
       -- Use the dialect-provided semantics, and substitute regions
-      let ret ← OpM.toTopM regionSemantics (S.semantics_op iop)
-      if not terminator then
-        match (res0, ret) with
-        | ([res], [⟨τ, v⟩]) =>
-            TopM.set τ res.fst v
-            return ret
-        | ([], []) =>
-            return ret
-        | _ =>
-          TopM.raiseUB s!"more than one result or unmatched result/expected pair: {op}"
-      else  -- TODO: refactor this code to be easier to read!
-        match (res0, ret) with
-        | ([res], [⟨τ, v⟩]) =>
-            TopM.set τ res.fst v
-            return ret
-        | _ => return ret
-
-
+      let ret ← OpM.toTopM (TopM.mapDenoteRegion regions0) (S.semantics_op iop)
+      match res0 with
+      | [] => pure ()
+      | [res] => match ret with
+          | [⟨τ, v⟩] => TopM.set τ res.fst v
+          | _ => TopM.raiseUB s!"denoteOp: expected 1 return value, got '{ret}'"
+      | _ => TopM.raiseUB s!"denoteOp: expected 0 or 1 results, got '{res0}'"
+      return ret
   -- denote a sequence of ops
-
 def denoteOps (stmts: List (Op Δ)): TopM Δ (TypedArgs Δ) :=
    match stmts with
    | [] => return  []
-   | [stmt] => denoteOp stmt (terminator := true)
+   | [stmt] => denoteOp stmt
    | (stmt :: stmts') => do
-        let _ ← denoteOp stmt (terminator := false)
+        let _ ← denoteOp stmt
         denoteOps stmts'
 
 def denoteRegion (rgn: Region Δ) (args: TypedArgs Δ):
@@ -504,7 +514,7 @@ def run! {Δ: Dialect α' σ' ε'}  {R} [Inhabited R]
 
 def run {Δ: Dialect α' σ' ε'} {R}
     (t: TopM  Δ R) (env: SSAEnv Δ):
-    Except String (R × SSAEnv Δ) :=
+    Except (String × SSAEnv Δ) (R × SSAEnv Δ) :=
   StateT.run t env
 
 -- The property for two programs to execute with no error and satisfy a
@@ -531,8 +541,7 @@ class Denote (δ: Dialect α σ ε) [S: Semantics δ]
 notation "⟦ " t " ⟧" => Denote.denote t
 
 instance DenoteOp (δ: Dialect α σ ε) [Semantics δ]: Denote δ Op where
-  denote op := denoteOp δ op (terminator := true)
-
+  denote op := denoteOp δ op
 -- This only works for single-BB regions with no arguments
 instance DenoteRegion (δ: Dialect α σ ε) [Semantics δ]: Denote δ Region where
   denote r := denoteRegion δ r []
@@ -540,6 +549,6 @@ instance DenoteRegion (δ: Dialect α σ ε) [Semantics δ]: Denote δ Region wh
 -- Not for regions because we need to specify the fuel
 
 @[simp] theorem Denote.denoteOp [Semantics δ]:
-  Denote.denote (self := DenoteOp δ) op = denoteOp δ op (terminator := true) := rfl
+  Denote.denote (self := DenoteOp δ) op = denoteOp δ op := rfl
 @[simp] theorem Denote.denoteRegion [Semantics δ]:
   Denote.denote (self := DenoteRegion δ) r = denoteRegion δ r [] := rfl
